Improved register allocation for ARM udiv and sdiv.
To accomodate hardware with and without support for integer divison,
the ARM backend imposes strong constraints on register allocation.

For hardware with support for integer division,
we lift this restriction.

For hardware without support for integer division,
instruction selection generates builtins.

arm/Asmexpand.ml
@@ -413,6 +413,16 @@ let expand_builtin_inline name args res =
   (* Optimization hint *)
   | "__builtin_unreachable", [], _ ->
      ()
+  (* Soft integer division *)
+  | "__aeabi_idiv", args , res ->
+     assert ((args,res) = ([BA(IR IR0); BA(IR IR1)] , BR (IR IR0)));
+     let id = intern_string "__aeabi_idiv" in
+     emit (Pblsymb(id,Builtins1.platform_builtin_sig Builtins1.BI_idiv))
+  | "__aeabi_uidiv", args , res ->
+     assert ((args,res) = ([BA(IR IR0); BA(IR IR1)] , BR (IR IR0)));
+     let id = intern_string "__aeabi_uidiv" in
+     emit (Pblsymb(id,Builtins1.platform_builtin_sig Builtins1.BI_uidiv))
+
   (* Catch-all *)
   | _ ->
       raise (Error ("unrecognized builtin " ^ name))
