arm/Builtins1.v
@@ -20,15 +20,40 @@ Require Import String Coqlib.
 Require Import AST Integers Floats Values.
 Require Import Builtins0.
 
-Inductive platform_builtin : Type := .
+Inductive platform_builtin : Type :=
+| BI_idiv
+| BI_uidiv.
 
 Local Open Scope string_scope.
 
 Definition platform_builtin_table : list (string * platform_builtin) :=
-  nil.
+  ("__aeabi_idiv", BI_idiv) ::   ("__aeabi_uidiv", BI_uidiv) :: nil.
 
 Definition platform_builtin_sig (b: platform_builtin) : signature :=
-  match b with end.
+  match b with
+  | BI_idiv | BI_uidiv => mksignature (Tint :: Tint :: nil) Tint cc_default
+  end.
+
+Definition divs (n1 n2: int) : option int :=
+  if Int.eq n2 Int.zero || Int.eq n1 (Int.repr Int.min_signed) && Int.eq n2 Int.mone then None else Some (Int.divs n1 n2).
+
+Remark divs_is_divs : forall n1 n2, Val.divs (Vint n1) (Vint n2) = option_map Vint (divs n1 n2).
+Proof.
+  unfold divs. simpl. intros.
+  destruct (Int.eq n2 Int.zero || Int.eq n1 (Int.repr Int.min_signed) && Int.eq n2 Int.mone);reflexivity.
+Qed.
+
+Definition divu (n1 n2: int) : option int :=
+  if Int.eq n2 Int.zero then None else Some (Int.divu n1 n2).
+
+Remark divu_is_divu : forall n1 n2, Val.divu (Vint n1) (Vint n2) = option_map Vint (divu n1 n2).
+Proof.
+  unfold divu. simpl. intros.
+  destruct (Int.eq n2 Int.zero);reflexivity.
+Qed.
 
 Definition platform_builtin_sem (b: platform_builtin) : builtin_sem (sig_res (platform_builtin_sig b)) :=
-  match b with end.
+  match b with
+  | BI_idiv => mkbuiltin_n2p Tint Tint (Tret Tint) divs
+  | BI_uidiv => mkbuiltin_n2p Tint Tint (Tret Tint) divu
+  end.
